semantics/semanticPrimitivesScript.sml
@@ -788,17 +788,19 @@ Datatype:
 End
 
 Definition dest_thunk_def:
-  dest_thunk [Loc _ n] st =
+  dest_thunk [Loc b n] st =
     (case store_lookup n st of
      | NONE => BadRef
-     | SOME (Thunk Evaluated v) => IsThunk Evaluated v
-     | SOME (Thunk NotEvaluated v) => IsThunk NotEvaluated v
+     | SOME (Thunk Evaluated v) =>
+         if b then BadRef else IsThunk Evaluated v
+     | SOME (Thunk NotEvaluated v) =>
+         if b then BadRef else IsThunk NotEvaluated v
      | SOME _ => NotThunk) ∧
   dest_thunk vs st = NotThunk
 End
 
 Definition update_thunk_def:
-  update_thunk [Loc _ n] st [v] =
+  update_thunk [Loc F n] st [v] =
     (case dest_thunk [v] st of
      | NotThunk => store_assign n (Thunk Evaluated v) st
      | _ => NONE) ∧
